Make encoding parameterized

src/lists.lean
@@ -1,66 +1,42 @@
 import polyfix
+import polysize
 import data.list.basic
 
 
-section list
+section foldl_lemmas
 
-def ptree_list_encoding_aux : polycodable (list ptree) :=
-{ encode := ptree.equiv_list.symm,
-  decode := ptree.equiv_list,
-  decode_encode := λ _, by simp,
-  polytime_decode := ⟨code.id, polytime_id, by simp⟩}
-
-local attribute [instance] ptree_list_encoding_aux
-
-open polycodable (encode decode)
+variables {α β γ : Type*} [inhabited γ]
 open part_eval (with_time eval)
 
-lemma polytime_fun.head : polytime_fun (@list.head ptree _) :=
-⟨code.left, polytime_left,
-by { intro x, cases x; simp [encode], refl, }⟩
+def foldl_step (f : α → γ → α) (x : list γ × α) : option (list γ × α) :=
+if x.1.empty then none else some (x.1.tail, f x.2 x.1.head)
 
-lemma polytime_fun.tail : polytime_fun (@list.tail ptree) :=
-⟨code.right, polytime_right,
-by { intro x, cases x; simp [encode], }⟩
-
-lemma polytime_fun.cons : polytime_fun₂ (@list.cons ptree) :=
-⟨code.id, polytime_id,
-by { intro x, dunfold polycodable.encode, cases x; simp [encode], }⟩
-
-variables {α β γ : Type*} [polycodable α] [polycodable β] [polycodable γ]
-def foldl_step (f : α → ptree → α) (x : list ptree × α) : option (list ptree × α) :=
-if x.1 = [] then none else some (x.1.tail, f x.2 x.1.head)
-
-lemma polytime_fun.foldl_step {f : β → α → ptree → α} (hf : polytime_fun₃ f) :
-  polytime_fun₂ (λ d, foldl_step (f d)) :=
-by { apply polytime_fun.ite, apply polytime_fun.eq_const, apply polytime_fun.comp polytime_fun.fst polytime_fun.snd, apply polytime_fun.const, apply polytime_fun.comp, apply polytime_fun.some, apply polytime_fun.pair, apply polytime_fun.comp, apply polytime_fun.tail, apply polytime_fun.comp, apply polytime_fun.fst, apply polytime_fun.snd, apply polytime_fun.comp₃ hf, apply polytime_fun.fst, apply polytime_fun.comp, apply polytime_fun.snd, apply polytime_fun.snd, apply polytime_fun.comp, apply polytime_fun.head, apply polytime_fun.comp, apply polytime_fun.fst, apply polytime_fun.snd, }
-
-theorem foldl_step_eval (f : α → ptree → α) (x : list ptree × α) (t : ℕ) :
-  eval (with_time (foldl_step f : list ptree × α →. option (list ptree × α)) (pfun.pure 1)) (t, x) =
+theorem foldl_step_eval (f : α → γ → α) (x : list γ × α) (t : ℕ) :
+  eval (with_time (foldl_step f : list γ × α →. option (list γ × α)) (pfun.pure 1)) (t, x) =
   part.some (t + x.1.length, [], x.1.foldl f x.2) :=
 begin
   rcases x with ⟨l, acc⟩, rw [part.eq_some_iff, part_eval.mem_eval],
   split, swap, { simp [with_time, foldl_step, pfun.pure], },
   induction l with hd tl ih generalizing acc t, { simp, },
-  have : some (t + 1, tl, f acc hd) ∈ with_time (foldl_step f : list ptree × α →. option (list ptree × α)) (pfun.pure 1) (t, hd :: tl, acc),
+  have : some (t + 1, tl, f acc hd) ∈ with_time (foldl_step f : list γ × α →. option (list γ × α)) (pfun.pure 1) (t, hd :: tl, acc),
   { simp [with_time, foldl_step, pfun.pure], },
   refine (part_eval.reaches_fwd this).trans _, simp at ⊢ ih, specialize ih (f acc hd) (t + 1),
   rw (show (t + (tl.length + 1) = t + 1 + tl.length), by ac_refl), exact ih,
 end
 
-theorem foldl_step_eval' (f : α → ptree → α) (x : list ptree × α) :
-  ([], x.1.foldl f x.2) ∈ eval (foldl_step f : list ptree × α →. option (list ptree × α)) x :=
+theorem foldl_step_eval' (f : α → γ → α) (x : list γ × α) :
+  ([], x.1.foldl f x.2) ∈ eval (foldl_step f : list γ × α →. option (list γ × α)) x :=
 begin
-  have : part_eval.frespects (with_time (foldl_step f : list ptree × α →. option (list ptree × α)) (pfun.pure 1)) (foldl_step f : list ptree × α →. option (list ptree × α)) _ :=
+  have : part_eval.frespects (with_time (foldl_step f : list γ × α →. option (list γ × α)) (pfun.pure 1)) (foldl_step f : list γ × α →. option (list γ × α)) _ :=
   part_eval.with_time_respects (by simp [pfun.pure]),
   have R := foldl_step_eval f x 0, simp [part.eq_some_iff] at R,
   exact this.of_eval R,
 end
 
-def foldl_inv (f : α → ptree → α) (x₀ : list ptree × α) : set (list ptree × α) :=
+def foldl_inv (f : α → γ → α) (x₀ : list γ × α) : set (list γ × α) :=
 {s | ∃ i ≤ x₀.1.length, s.1 = x₀.1.drop i ∧ s.2 = (x₀.1.take i).foldl f x₀.2}
 
-theorem foldl_step_invariant (f : α → ptree → α) (x₀) ⦃x y : list ptree × α⦄ (hx : x ∈ foldl_inv f x₀) (hy : some y = foldl_step f x) :
+theorem foldl_step_invariant (f : α → γ → α) (x₀) ⦃x y : list γ × α⦄ (hx : x ∈ foldl_inv f x₀) (hy : some y = foldl_step f x) :
   y ∈ foldl_inv f x₀ :=
 begin 
   rcases x with ⟨x₁, x₂⟩, rcases x₀ with ⟨l₀, acc₀⟩,
@@ -68,7 +44,7 @@ begin
   rcases hx with ⟨i, H, rfl, rfl⟩,
   by_cases l₀.length ≤ i,
   { simp [h, foldl_step] at hy, contradiction, },
-  simp [foldl_step, list.drop_eq_nil_iff_le, h] at hy,
+  simp [foldl_step, list.empty_iff_eq_nil, list.drop_eq_nil_iff_le, h] at hy,
   refine ⟨i+1, _, _, _⟩,
   { rwa [nat.succ_le_iff, lt_iff_not_le], },
   { rw hy, simp [← list.drop_one], congr' 1, ac_refl, },
@@ -78,7 +54,7 @@ begin
   rw [list.drop_eq_nth_le_cons h, list.take_succ, list.nth_le_nth h], simp [option.to_list],
 end
 
-theorem foldl_step_eval_inv (f : α → ptree → α) (x : list ptree × α) :
+theorem foldl_step_eval_inv (f : α → γ → α) (x : list γ × α) :
   x.1.length + 1 ∈ part_eval.time_iter (pfun.res (foldl_step f) (foldl_inv f x)) (pfun.pure 1) x :=
 begin
   rw [← pfun.coe_res_inter, ← part_eval.time_iter_invariant],
@@ -88,23 +64,66 @@ begin
   use 0, simp,
 end
 
+lemma foldl_cons_eq_reverse {δ : Type*} (l : list δ) (xs : list δ) : 
+  list.foldl (λ a b, b :: a) xs l = l.reverse ++ xs :=
+by { induction l with hd tl ih generalizing xs, { simp, }, simp [ih], }
+
+lemma foldr_eq_map {δ ε} (l : list δ) (f : δ → ε) (xs : list ε) : l.foldr (λ a b, f a :: b) xs = (l.map f) ++ xs :=
+by { induction l, { simp, }, simpa, }
+
+end foldl_lemmas
+
+section list
+variables {α β γ : Type*} [polycodable α] [polycodable β] [polycodable γ]
+open polycodable (encode decode)
+
+variable (H_enc : polytime_fun (λ l : ptree, ptree.equiv_list.symm $ l.equiv_list.map (encode ∘ (@decode γ _))))
+
+def inh : inhabited γ := ⟨decode ptree.nil⟩ 
+local attribute [instance] inh
+
+include H_enc
+-- List encoding aux; used very frequently, so better have a short name
+def lea : polycodable (list γ) :=
+{ encode := λ l, ptree.equiv_list.symm (l.map encode),
+  decode := λ v, v.equiv_list.map decode,
+  decode_encode := λ _, by simp,
+  polytime_decode := by { rw polytime_fun_iff', simpa using H_enc, } }
+
+lemma lea_encode (x : list γ) : by haveI := lea H_enc; exact encode x = ptree.equiv_list.symm (x.map encode) := rfl
+lemma lea_decode (x : ptree) : by haveI := lea H_enc; exact (decode x : list γ) = x.equiv_list.map decode := rfl
+
+
+open part_eval (with_time eval)
+
+lemma polytime_fun.head : by haveI := lea H_enc; exact polytime_fun (@list.head γ _) :=
+by { rw polytime_fun_iff'', use [code.left, polytime_left], intro x, cases x; simp [lea_encode], refl, }
+
+lemma polytime_fun.tail : by haveI := lea H_enc; exact polytime_fun (@list.tail γ) :=
+⟨code.right, polytime_right,
+by { intro x, cases x; simp [lea_decode, lea_encode], }⟩
+
+lemma polytime_fun.cons : by haveI := lea H_enc; exact polytime_fun₂ (@list.cons γ) :=
+⟨code.id, polytime_id,
+by { intro x, dunfold polycodable.encode, cases x; simp [lea_encode], }⟩
+
+lemma polytime_fun.is_empty : by haveI := lea H_enc; exact polytime_fun (@list.empty γ) :=
+by { letI := lea H_enc, classical, convert_to polytime_fun (λ l : list γ, (l = [] : bool)), { ext x, cases x; simp, }, apply polytime_fun.eq_const polytime_fun.id, }
+
+lemma polytime_fun.foldl_step {f : β → α → γ → α} (hf : polytime_fun₃ f) :
+  (by haveI := lea H_enc; exact (polytime_fun₂ (λ d, foldl_step (f d)))) :=
+by { letI := lea H_enc, apply polytime_fun.ite, simp, apply polytime_fun.comp, apply polytime_fun.is_empty, apply polytime_fun.comp polytime_fun.fst polytime_fun.snd, apply polytime_fun.const, apply polytime_fun.comp, apply polytime_fun.some, apply polytime_fun.pair, apply polytime_fun.comp, apply polytime_fun.tail, apply polytime_fun.comp, apply polytime_fun.fst, apply polytime_fun.snd, apply polytime_fun.comp₃ hf, apply polytime_fun.fst, apply polytime_fun.comp, apply polytime_fun.snd, apply polytime_fun.snd, apply polytime_fun.comp, apply polytime_fun.head, apply polytime_fun.comp, apply polytime_fun.fst, apply polytime_fun.snd, }
+
 section encode_sizeof
 
+@[simp] lemma encode_sizeof_nil : by haveI := lea H_enc; exact (encode ([] : list γ)).sizeof = 1 :=
+by simp [lea_encode]
+@[simp] lemma encode_sizeof_cons (a : γ) (b : list γ) :
+  by haveI := lea H_enc; exact (encode (a :: b)).sizeof = 1 + (encode a).sizeof + (encode b).sizeof :=
+by simp [lea_encode]
 
-open polycodable (encode)
-
-@[simp] lemma encode_sizeof_ptree (x : ptree) : (encode x).sizeof = x.sizeof := rfl
-@[simp] lemma encode_sizeof_nil : (encode ([] : list ptree)).sizeof = 1 :=
-by simp [encode]
-@[simp] lemma encode_sizeof_cons (a : ptree) (b : list ptree) :
-  (encode (a :: b)).sizeof = 1 + (encode a).sizeof + (encode b).sizeof :=
-by simp [encode]
-lemma one_le_encode_sizeof (x : α) :
-  1 ≤ (encode x).sizeof :=
-by { cases (encode x); simp, linarith only, }
-
-lemma encode_sizeof_le_of_mem {l : list ptree} {x : ptree} (hx : x ∈ l) :
-  x.sizeof ≤ (encode l).sizeof :=
+lemma encode_sizeof_le_of_mem {l : list γ} {x : γ} (hx : x ∈ l) :
+  by haveI := lea H_enc; exact (encode x).sizeof ≤ (encode l).sizeof :=
 begin
   induction l with hd tl ih, { simp at hx, contradiction, },
   rcases ((list.mem_cons_iff _ _ _).mp hx) with rfl|h; simp,
@@ -112,112 +131,63 @@ begin
   linarith only [ih h],
 end
 
-@[simp] lemma encode_sizeof_pair (a : α) (b : β) : (encode (a, b)).sizeof = (encode a).sizeof + (encode b).sizeof + 1 :=
-by { simp [encode], ac_refl, }
-
-@[simp] lemma encode_sizeof_append (a b : list ptree) :
+@[simp] lemma encode_sizeof_append (a b : list γ) : by haveI := lea H_enc; exact
   ((encode (a ++ b)).sizeof : ℤ) = ((encode a).sizeof : ℤ) + (encode b).sizeof - 1 :=
 by { induction a with hd tl ih, { simp, }, simp [ih], ring, }
 
-lemma encode_sizeof_le_of_infix {a b : list ptree} (h : a <:+: b) :
+lemma encode_sizeof_le_of_infix {a b : list γ} (h : a <:+: b) : by haveI := lea H_enc; exact
   (encode a).sizeof ≤ (encode b).sizeof :=
 begin
-  rcases h with ⟨s, t, rfl⟩,
+  letI := lea H_enc, rcases h with ⟨s, t, rfl⟩,
   have i₁ := one_le_encode_sizeof s, have i₂ := one_le_encode_sizeof t,
   zify at *, simp, linarith,
 end
 
-lemma encode_list_sizeof (l : list ptree) : (encode l).sizeof = (l.map ptree.sizeof).sum + l.length + 1 :=
+lemma encode_list_sizeof (l : list γ) : by haveI := lea H_enc; exact 
+  (encode l).sizeof = (l.map (λ x, (encode x).sizeof)).sum + l.length + 1 :=
 by { induction l with hd tl ih, { simp, }, simp [ih], ac_refl, }
 
-@[simp] lemma encode_sizeof_reverse (l : list ptree) :
+@[simp] lemma encode_sizeof_reverse (l : list γ) : by haveI := lea H_enc; exact
   (encode l.reverse).sizeof = (encode l).sizeof :=
 by { simp [encode_list_sizeof, list.sum_reverse], }
 
-lemma len_le_encode_sizeof (a : list ptree) :
+lemma len_le_encode_sizeof (a : list γ) : by haveI := lea H_enc; exact
   a.length + 1 ≤ (encode a).sizeof :=
 by { induction a with hd tl ih, { simp, }, simp, linarith, }
 
-
-def polysize_fun (f : α → β) : Prop :=
-∃ p : polynomial ℕ, ∀ (x : α), (encode (f x)).sizeof ≤ p.eval (encode x).sizeof
-
-lemma polysize_of_polytime_fun {f : α → β} (hf : polytime_fun f) :
-  polysize_fun f :=
+lemma polysize_fun_map_polysize {f : β → γ → γ} (hf : polysize_fun₂ f) : by haveI := lea H_enc; exact
+  polysize_fun₂ (λ (s : β) (l : list γ), l.map (f s)) :=
 begin
-  rcases hf with ⟨c, ⟨p, hp⟩, sc⟩, use p,
-  intro x, specialize sc x, rw part.eq_some_iff at sc,
-  rcases hp (encode x) with ⟨t, ht, t_le⟩,
-  exact (eval_sizeof_le_time sc ht).trans t_le,
-end
-
-lemma polysize_fun.comp {g : β → γ} {f : α → β} (hg : polysize_fun g) (hf : polysize_fun f) :
-  polysize_fun (g ∘ f) :=
-begin
-  rcases hf with ⟨pf, hpf⟩, rcases hg with ⟨pg, hpg⟩,
-  use pg.comp pf, intro x, simp,
-  refine (hpg _).trans (monotone_polynomial_nat _ _),
-  apply hpf,
-end
-
-section
-variables {δ ε : Type*} [polycodable δ] [polycodable ε]
-
-def polysize_fun₂ (f : α → β → γ) : Prop := polysize_fun (function.uncurry f)
-lemma polysize₂_of_polytime₂ {f : α → β → γ} (hf : polytime_fun₂ f) : polysize_fun₂ f :=
-polysize_of_polytime_fun hf
-
-lemma polysize_fun.pair {f : α → β} {g : α → γ} (hf : polysize_fun f) (hg : polysize_fun g) :
-  polysize_fun (λ s, (f s, g s)) :=
-by { cases hf with pf hpf, cases hg with pg hpg, use pf + pg + 1, intro x, simpa using add_le_add (hpf _) (hpg _), }
-
-lemma polysize_fun.comp₂ {f : α → β → γ} {g : δ → α} {h : δ → β} (hf : polysize_fun₂ f) (hg : polysize_fun g) (hh : polysize_fun h) :
-  polysize_fun (λ s, f (g s) (h s)) :=
-polysize_fun.comp hf (polysize_fun.pair hg hh)
-
-
-def polysize_fun₃ (f : α → β → γ → δ) : Prop :=
-polysize_fun (λ a : α × β × γ, f a.1 a.2.1 a.2.2)
-lemma polysize₃_of_polytime₃ {f : α → β → γ → δ} (hf : polytime_fun₃ f) : polysize_fun₃ f :=
-polysize_of_polytime_fun hf
-lemma polysize_fun.comp₃ {f : α → β → γ → δ} {g : ε → α} {h : ε → β} {i : ε → γ}
-  (hf : polysize_fun₃ f) (hg : polysize_fun g) (hh : polysize_fun h) (hi : polysize_fun i) :
-  polysize_fun (λ s, f (g s) (h s) (i s)) :=
-polysize_fun.comp hf (polysize_fun.pair hg (polysize_fun.pair hh hi))
-
-end
-
-lemma polysize_fun_map_polysize {f : β → ptree → ptree} (hf : polysize_fun₂ f) :
-  polysize_fun₂ (λ (s : β) (l : list ptree), l.map (f s)) :=
-begin
+  letI := lea H_enc,
   rcases hf with ⟨p, hp⟩,
   use (polynomial.monomial 1 1) * p + (polynomial.monomial 1 1) + 1, rintro ⟨s, l⟩, dsimp only,
   conv_lhs { rw encode_list_sizeof, },
   simp, mono,
-  { refine (list.sum_le_card_nsmul (l.map (ptree.sizeof ∘ f s)) (p.eval $ (encode s).sizeof + (encode l).sizeof + 1) _).trans _, 
+  { refine (list.sum_le_card_nsmul (l.map (λ x, (encode (f s x)).sizeof)) (p.eval $ (encode s).sizeof + (encode l).sizeof + 1) _).trans _, 
     { intros x hx, simp at hx, rcases hx with ⟨x, hx, rfl⟩, refine (hp ⟨s, x⟩).trans _,
-      apply monotone_polynomial_nat, simpa using encode_sizeof_le_of_mem hx, },
-    simp, apply mul_le_mul_right', refine (nat.le_succ _).trans ((len_le_encode_sizeof l).trans _), linarith only, },
-  refine (nat.le_succ _).trans ((len_le_encode_sizeof l).trans _), linarith only,
+      apply monotone_polynomial_nat, simpa using encode_sizeof_le_of_mem H_enc hx, },
+    simp, apply mul_le_mul_right', refine (nat.le_succ _).trans ((len_le_encode_sizeof H_enc l).trans _), linarith only, },
+  refine (nat.le_succ _).trans ((len_le_encode_sizeof H_enc l).trans _), linarith only,
 end
 
 end encode_sizeof
 
-theorem polytime_fun.foldl_aux {f : β → α → ptree → α} {l : β → list ptree} {acc : β → α} 
-  (hf : polytime_fun₃ f) (hl : polytime_fun l) (hacc : polytime_fun acc) 
-  (hs : polysize_fun₃ (λ (s : β) (x : α) (l : list ptree), l.foldl (f s) x)) :
+theorem polytime_fun.foldl_aux {f : β → α → γ → α} {l : β → list γ} {acc : β → α} 
+  (hf : polytime_fun₃ f) (hl : by haveI := lea H_enc; exact polytime_fun l) (hacc : polytime_fun acc) 
+  (hs : by haveI := lea H_enc; exact polysize_fun₃ (λ (s : β) (x : α) (l : list γ), l.foldl (f s) x)) :
   polytime_fun (λ s, (l s).foldl (f s) (acc s)) :=
 begin
-  suffices : polytime_fun₃ (λ s (L : list ptree) (a : α), (@list.nil ptree, L.foldl (f s) a)),
+  letI := lea H_enc,
+  suffices : polytime_fun₃ (λ s (L : list γ) (a : α), (@list.nil γ, L.foldl (f s) a)),
   { have pf : polytime_fun (λ s, (s, l s, acc s)) := polytime_fun.pair polytime_fun.id (polytime_fun.pair hl hacc),
     exact polytime_fun.comp polytime_fun.snd (polytime_fun.comp this pf), },
   cases hs with ps hps,
-  refine polytime_fun.eval (λ s : β, foldl_step (f s)) (λ (s : β) (x : list ptree × α), ([], x.1.foldl (f s) x.2))
+  refine polytime_fun.eval (λ s : β, foldl_step (f s)) (λ (s : β) (x : list γ × α), ([], x.1.foldl (f s) x.2))
     _ (polynomial.monomial 1 1) (ps + polynomial.monomial 1 1) _ _,
-  { exact polytime_fun.foldl_step hf, },
+  { exact polytime_fun.foldl_step H_enc hf, },
   { rintros s ⟨l₀, a₀⟩, simp, apply foldl_step_eval', },
   rintros S ⟨l₀, a₀⟩, use l₀.length + 1, split,
-  { simp, linarith only [len_le_encode_sizeof l₀], },
+  { simp, linarith only [len_le_encode_sizeof H_enc l₀], },
   apply part_eval.time_iter_mono _ (foldl_step_eval_inv (f S) (l₀, a₀)),
   rintros ⟨l₁, a₁⟩ y, simp [pfun.mem_res], rintros h₁ h₂, refine ⟨_, h₂⟩,
   simp [foldl_inv] at h₁, rcases h₁ with ⟨i, hi, rfl, rfl⟩,
@@ -225,82 +195,61 @@ begin
   { apply encode_sizeof_le_of_infix, exact (l₀.drop_suffix i).is_infix, },
   apply le_add_left, simp,
   specialize hps ⟨S, a₀, l₀.take i⟩, simp at hps, refine hps.trans (monotone_polynomial_nat _ _),
-  ring_nf, simp, exact encode_sizeof_le_of_infix (l₀.take_prefix i).is_infix,
+  ring_nf, simp, exact encode_sizeof_le_of_infix H_enc (l₀.take_prefix i).is_infix,
 end
 
-lemma foldl_cons_eq_reverse {δ : Type*} (l : list δ) (xs : list δ) : 
-  list.foldl (λ a b, b :: a) xs l = l.reverse ++ xs :=
-by { induction l with hd tl ih generalizing xs, { simp, }, simp [ih], }
-
-theorem polytime_fun.reverse_aux : polytime_fun (@list.reverse ptree) :=
+theorem polytime_fun.reverse_aux : by haveI := lea H_enc; exact
+  polytime_fun (@list.reverse γ) :=
 begin
-  convert_to polytime_fun (λ l : list ptree, l.foldl (λ acc hd, hd :: acc) []),
+  letI := lea H_enc,
+  convert_to polytime_fun (λ l : list γ, l.foldl (λ acc hd, hd :: acc) []),
   { ext l : 1, simp [foldl_cons_eq_reverse], },
   apply polytime_fun.foldl_aux,
-  { simp only [polytime_fun₃], apply polytime_fun.comp₂ polytime_fun.cons, apply polytime_fun.comp polytime_fun.snd polytime_fun.snd, apply polytime_fun.comp polytime_fun.fst polytime_fun.snd, },
+  { simp only [polytime_fun₃], apply polytime_fun.comp₂ (polytime_fun.cons H_enc), apply polytime_fun.comp polytime_fun.snd polytime_fun.snd, apply polytime_fun.comp polytime_fun.fst polytime_fun.snd, },
   { exact polytime_fun.id, }, { exact polytime_fun.const _, },
   simp [foldl_cons_eq_reverse], use polynomial.monomial 1 1,
   rintro ⟨a, b, c⟩, zify, simp, linarith only,
 end
 
-theorem polytime_fun.foldr_aux {f : β → ptree → α → α} {l : β → list ptree} {acc : β → α} 
-  (hf : polytime_fun₃ f) (hl : polytime_fun l) (hacc : polytime_fun acc) 
-  (hs : polysize_fun₃ (λ (s : β) (x : α) (l : list ptree), l.foldr (f s) x)) :
+theorem polytime_fun.foldr_aux {f : β → γ → α → α} {l : β → list γ} {acc : β → α} 
+  (hf : polytime_fun₃ f) (hl : by haveI := lea H_enc; exact polytime_fun l) (hacc : polytime_fun acc) 
+  (hs : by haveI := lea H_enc; exact polysize_fun₃ (λ (s : β) (x : α) (l : list γ), l.foldr (f s) x)) :
   polytime_fun (λ s, (l s).foldr (f s) (acc s)) :=
 begin
+  letI := lea H_enc,
   simp only [← list.foldl_reverse], apply polytime_fun.foldl_aux,
   { apply polytime_fun.comp₃ hf polytime_fun.fst; apply polytime_fun.comp, any_goals { exact polytime_fun.snd, }, exact polytime_fun.fst, },
-  { apply polytime_fun.comp polytime_fun.reverse_aux hl, },
+  { apply polytime_fun.comp (polytime_fun.reverse_aux H_enc) hl, },
   { exact hacc, },
   simp only [← list.foldr_reverse],
-  suffices : polysize_fun (λ xls : β × α × list ptree, (xls.1, xls.2.1, xls.2.2.reverse)),
+  suffices : polysize_fun (λ xls : β × α × list γ, (xls.1, xls.2.1, xls.2.2.reverse)),
   { exact polysize_fun.comp hs this, }, apply polysize_of_polytime_fun,
   apply polytime_fun.pair polytime_fun.fst, apply polytime_fun.pair; apply polytime_fun.comp,
-  exacts [polytime_fun.fst, polytime_fun.snd, polytime_fun.reverse_aux, polytime_fun.comp polytime_fun.snd polytime_fun.snd],
+  exacts [polytime_fun.fst, polytime_fun.snd, (polytime_fun.reverse_aux H_enc), polytime_fun.comp polytime_fun.snd polytime_fun.snd],
 end
 
-lemma foldr_eq_map {δ ε} (l : list δ) (f : δ → ε) (xs : list ε) : l.foldr (λ a b, f a :: b) xs = (l.map f) ++ xs :=
-by { induction l, { simp, }, simpa, }
 
-lemma polysize_fun.append : polysize_fun₂ (@list.append ptree) :=
+lemma polysize_fun.append : by haveI := lea H_enc; exact
+  polysize_fun₂ (@list.append γ) :=
 ⟨polynomial.monomial 1 1,
 by { rintro ⟨a, b⟩, zify, simp [list.append_eq_has_append], linarith, }⟩
 
-theorem polytime_fun.map_aux {f : β → ptree → ptree} {l : β → list ptree} (hf : polytime_fun₂ f) (hl : polytime_fun l) :
+theorem polytime_fun.map_aux {f : β → γ → γ} {l : β → list γ}
+  (hf : polytime_fun₂ f)
+  (hl : by haveI := lea H_enc; exact polytime_fun l) : by haveI := lea H_enc; exact
   polytime_fun (λ s, (l s).map (f s)) :=
 begin
+  letI := lea H_enc,
   convert_to polytime_fun (λ s : β, (l s).foldr (λ a b, f s a :: b) []),
   { ext s : 1, simp [foldr_eq_map], },
   apply polytime_fun.foldr_aux,
-  { apply polytime_fun.comp₂ polytime_fun.cons, apply polytime_fun.comp₂ hf, exact polytime_fun.fst, all_goals { apply polytime_fun.comp, }, any_goals { apply polytime_fun.snd, }, apply polytime_fun.fst, },
+  { apply polytime_fun.comp₂ (polytime_fun.cons H_enc), apply polytime_fun.comp₂ hf, exact polytime_fun.fst, all_goals { apply polytime_fun.comp, }, any_goals { apply polytime_fun.snd, }, apply polytime_fun.fst, },
   { exact hl, }, { apply polytime_fun.const, },
   simp only [foldr_eq_map],
-  apply polysize_fun.comp₂ polysize_fun.append,
-  { refine polysize_fun.comp (polysize_fun_map_polysize (polysize₂_of_polytime₂ hf)) (_ : polysize_fun (λ s : β × list ptree × list ptree, (s.1, s.2.2))), 
+  apply polysize_fun.comp₂ (polysize_fun.append H_enc),
+  { refine polysize_fun.comp (polysize_fun_map_polysize H_enc (polysize₂_of_polytime₂ hf)) (_ : polysize_fun (λ s : β × list γ × list γ, (s.1, s.2.2))), 
     apply polysize_of_polytime_fun, apply polytime_fun.pair polytime_fun.fst, apply polytime_fun.comp polytime_fun.snd polytime_fun.snd, },
   apply polysize_of_polytime_fun, apply polytime_fun.comp polytime_fun.fst polytime_fun.snd,
 end
-
-local attribute [-instance] ptree_list_encoding_aux
-
-instance : polycodable (list α) :=
-@polycodable.mk' (list ptree) ptree_list_encoding_aux (list α)
-(list.map encode)
-(list.map decode)
-(by simp)
-begin
-  simp, apply polytime_fun.map_aux, swap,
-  { apply polytime_fun.id, },
-  simp only [polytime_fun₂, function.uncurry], apply polytime_fun.comp,
-  apply polytime_fun.comp polytime_fun.encode polytime_fun.decode', apply polytime_fun.snd,
-end
-
-lemma encode_list_ptree_eq (l : list ptree) :
-  encode l = ptree.equiv_list.symm l :=
-by { simp [encode], }
-
-private lemma polytime_fun_list_ptree_iff (f : α → list ptree → β) :
-  polytime_fun₂ f ↔ @polytime_fun₂ _ _ _ _ ptree_list_encoding_aux _ f :=
-by { simp [polytime_fun₂, polytime_fun, function.uncurry, encode], }
 
 end list
